theories/channel/proofmode.v
@@ -489,3 +489,12 @@ Tactic Notation "wp_new_chan" constr(prot) "as"
        "(" simple_intropattern(c1) simple_intropattern(c2) ")" constr(pat) :=
   wp_smart_apply (new_chan_spec prot); [done|];
   iIntros (c1); iIntros (c2); iIntros pat.
+
+Tactic Notation "wp_fork_chan" constr(prot) "as"
+       simple_intropattern(c1) constr(pat1) "and" simple_intropattern(c2) constr(pat2) :=
+  wp_smart_apply (fork_chan_spec prot); [iIntros (c1); iIntros pat1|
+                                         iIntros (c2); iIntros pat2].
+
+Tactic Notation "wp_fork_chan" constr(prot) :=
+  wp_smart_apply (fork_chan_spec prot).
+
